src/SlabsFree.fst
@@ -57,7 +57,6 @@ let deallocate_slab_aux_cond
     r == is_empty size_class v0
   )
   =
-  admit ();
   assert (t_of (A.varray md) == Seq.lseq U64.t 4);
   let md_as_seq : G.erased (Seq.lseq U64.t 4)
     = elim_slab_vprop size_class md arr in
